Machine run complete

theories/machine_run.v
@@ -3,7 +3,7 @@ From iris.program_logic Require Import language.
 From cap_machine Require Import machine_parameters machine_base cap_lang.
 
 Section machine_run.
-  Context `{MachineParameters}.
+  Context {MP:MachineParameters}.
 
   (* The operational semantics as an interpreter: this effectively "runs" the
     machine until it fails or halts (or we run out of fuel). *)
@@ -100,6 +100,280 @@ Section machine_run.
         eapply step_atomic with (t1:=[]). 1,2: reflexivity. cbn.
         eapply ectx_language.Ectx_step with (K:=[]). 1,2: reflexivity. cbn.
         econstructor. cbn. apply Hc. } }
+  Qed.
+
+  Fixpoint depth expr :=
+    match expr with
+    | Instr _ => 0
+    | Seq expr => S (depth expr)
+    end.
+
+  Lemma fill_depth K cf :
+    depth (ectx_language.fill K cf) = length K + depth cf.
+  Proof.
+    generalize cf. clear cf.
+    induction K.
+    reflexivity. intros cf.
+    destruct a. simpl.
+    rewrite (IHK (Seq cf)).
+    simpl. lia.
+  Qed.
+
+  Lemma fill_seq_seq {cf K cf'} :
+    Seq (Instr cf) = ectx_language.fill K (Seq (Instr cf')) ->
+    K = [] /\ cf = cf'.
+  Proof.
+    intros H.
+    apply (f_equal depth) in H as Hd.
+    rewrite fill_depth in Hd. simpl in Hd.
+    assert (Hk : K = []).
+    apply nil_length_inv.
+    apply (Nat.add_cancel_r _ _ 1).
+    symmetry. simpl. exact Hd.
+    split. exact Hk.
+    rewrite Hk in H. inversion H. reflexivity.
+  Qed.
+
+  Lemma fill_seq_instr {cf k cf'} :
+    Seq (Instr cf) = ectx_language.fill k (Instr cf') ->
+    k = [ SeqCtx ] /\ cf = cf'.
+  Proof.
+    intros H.
+    apply (f_equal depth) in H as Hd.
+    rewrite fill_depth in Hd. simpl in Hd.
+    destruct k; simpl in Hd. lia.
+    apply (inj S) in Hd. rewrite Nat.add_0_r in Hd.
+    assert (Hk : k = []).
+    apply nil_length_inv. symmetry. exact Hd.
+    rewrite Hk. destruct e.
+    split. reflexivity. rewrite Hk in H. inversion H. reflexivity.
+  Qed.
+
+  Lemma fill_simpl {cf K e} :
+    Seq (Instr cf) = ectx_language.fill K e ->
+    e = Instr cf \/ e = Seq (Instr cf).
+  Proof.
+    intros H.
+    apply (f_equal depth) in H as Hd.
+    rewrite fill_depth in Hd.
+    destruct e; simpl in Hd.
+    left.
+    destruct K; simpl in Hd. discriminate.
+    assert (Hk : K = []).
+    apply nil_length_inv.
+    apply (inj S) in Hd. rewrite Nat.add_0_r in Hd.
+    symmetry. apply Hd. rewrite Hk in H.
+    destruct e. simpl in H. inversion H. reflexivity.
+    right. assert (Hk : K = []).
+    apply nil_length_inv. rewrite Nat.add_succ_r in Hd.
+    apply (inj S) in Hd. symmetry in Hd.
+    apply Nat.eq_add_0 in Hd. destruct Hd. assumption.
+    rewrite Hk in H. simpl in H. inversion H. reflexivity.
+  Qed.
+
+  Lemma fill_instr {c k e}:
+    Instr c = ectx_language.fill k e -> Instr c = e.
+  Proof.
+    intros H. apply (f_equal depth) in H as Hd.
+    rewrite fill_depth in Hd. simpl in Hd.
+    assert (Hk : k = []).
+    apply nil_length_inv. symmetry in Hd. apply Nat.eq_add_0 in Hd.
+    destruct Hd as [Hd _]. apply Hd.
+    rewrite Hk in H. simpl in H. inversion H. reflexivity.
+  Qed.
+
+  Lemma singleton_app_cons {A:Type} {e e':A} {t t':list A} :
+    [e] = t ++ e' :: t' -> e = e' /\ t = [] /\ t' = [].
+  Proof.
+    intros H. symmetry in H. apply app_singleton in H.
+    destruct H as [[Ht Het]|[_ Habsurd]].
+    2: discriminate.
+    apply (inj2 cons) in Het as [l r]. auto.
+  Qed.
+
+  Lemma erased_step_halted {cf φ φ'}:
+    rtc erased_step ([Instr Halted], φ) ([Instr cf], φ') ->
+    cf = Halted.
+  Proof.
+    intros Hstep.
+    rewrite erased_steps_nsteps in Hstep.
+    destruct Hstep as [n [ks Hstep]].
+    revert Hstep. generalize ks. clear ks.
+    induction n.
+    intros. inversion Hstep. reflexivity.
+    intros. inversion Hstep.
+    inversion H0.
+    apply pair_equal_spec in H5 as [H5 Hφ].
+    apply singleton_app_cons in H5 as [He [Ht1 Ht2]].
+    rewrite -He in H7.
+    inversion H7. simpl in K, e1', e2'.
+    apply fill_instr in H5.
+    rewrite -H5 in H9; inversion H9.
+  Qed.
+
+  Lemma erased_step_failed {cf φ φ'}:
+    rtc erased_step ([Instr Failed], φ) ([Instr cf], φ') ->
+    cf = Failed.
+  Proof.
+    intros Hstep.
+    rewrite erased_steps_nsteps in Hstep.
+    destruct Hstep as [n [ks Hstep]].
+    revert Hstep. generalize ks. clear ks.
+    induction n.
+    intros. inversion Hstep. reflexivity.
+    intros. inversion Hstep.
+    inversion H0.
+    apply pair_equal_spec in H5 as [H5 Hφ].
+    apply singleton_app_cons in H5 as [He [Ht1 Ht2]].
+    rewrite -He in H7.
+    inversion H7. simpl in K, e1', e2'.
+    apply fill_instr in H5.
+    rewrite -H5 in H9; inversion H9.
+  Qed.
+
+  Lemma erased_step_seq_halted {cf φ φ'}:
+    rtc erased_step ([Seq (Instr Halted)], φ) ([Instr cf], φ') ->
+    cf = Halted.
+  Proof.
+    intros Hstep.
+    rewrite erased_steps_nsteps in Hstep.
+    destruct Hstep as [n [ks Hstep]].
+    inversion Hstep.
+    inversion H.
+    apply pair_equal_spec in H5 as [H5 Hφ].
+    apply singleton_app_cons in H5 as [He [Ht1 Ht2]].
+    rewrite -He in H7.
+    inversion H7. simpl in K, e1', e2'.
+    destruct (fill_simpl H5) as [He1 | He1];
+    rewrite He1 in H9; inversion H9.
+    rewrite He1 in H5. apply fill_seq_seq in H5 as [HK _].
+    rewrite HK -H13 in H8. simpl in H8.
+    rewrite H8 Ht1 Ht2 -H15 -H14 -Hφ in H6. simpl in H6.
+    rewrite H6 in H0.
+    apply (ex_intro (fun κs => nsteps n0 ([Instr Halted], φ) κs ([Instr cf], φ')) κs) in H0.
+    apply (ex_intro (fun n0 => ∃ κs, nsteps n0 ([Instr Halted], φ) κs ([Instr cf], φ')) n0) in H0.
+    rewrite -erased_steps_nsteps in H0.
+    apply (erased_step_halted H0).
+  Qed.
+
+  Lemma erased_step_seq_failed {cf φ φ'}:
+    rtc erased_step ([Seq (Instr Failed)], φ) ([Instr cf], φ') ->
+    cf = Failed.
+  Proof.
+    intros Hstep.
+    rewrite erased_steps_nsteps in Hstep.
+    destruct Hstep as [n [ks Hstep]].
+    inversion Hstep.
+    inversion H.
+    apply pair_equal_spec in H5 as [H5 Hφ].
+    apply singleton_app_cons in H5 as [He [Ht1 Ht2]].
+    rewrite -He in H7.
+    inversion H7. simpl in K, e1', e2'.
+    destruct (fill_simpl H5) as [He1 | He1];
+    rewrite He1 in H9; inversion H9.
+    rewrite He1 in H5. apply fill_seq_seq in H5 as [HK _].
+    rewrite HK -H13 in H8. simpl in H8.
+    rewrite H8 Ht1 Ht2 -H15 -H14 -Hφ in H6. simpl in H6.
+    rewrite H6 in H0.
+    apply (ex_intro (fun κs => nsteps n0 ([Instr Failed], φ) κs ([Instr cf], φ')) κs) in H0.
+    apply (ex_intro (fun n0 => ∃ κs, nsteps n0 ([Instr Failed], φ) κs ([Instr cf], φ')) n0) in H0.
+    rewrite -erased_steps_nsteps in H0.
+    apply (erased_step_failed H0).
+  Qed.
+
+  Lemma machine_run_complete cf (φ φ': ExecConf) cf':
+    rtc erased_step ([Seq (Instr cf)], φ) ([Instr cf'], φ') ->
+    ∃ fuel, machine_run fuel (cf, φ) = Some cf'.
+  Proof.
+    intros Hstep. rewrite rtc_list in Hstep.
+    destruct Hstep as [l [Hhd [Htl Hstep]]].
+    revert Hhd Htl Hstep. revert φ φ' cf cf'.
+    induction l; intros. discriminate Hhd.
+    apply Some_inj in Hhd.
+    destruct l as [|b l].
+    apply Some_inj in Htl. rewrite Hhd in Htl. discriminate.
+
+    specialize (Hstep 0 a b eq_refl eq_refl) as Hstep'.
+    destruct Hstep' as [k Hstep'].
+    inversion Hstep' as [e1 σ1 e2 σ2 extra t1 t2 Ha Hb Hstep''].
+    inversion Hstep'' as [K e1' e2' He1 He2 Hstep''']. simpl in K, e1', e2'.
+    rewrite Hhd in Ha.
+    apply pair_equal_spec in Ha as [Ha Hφ].
+    apply singleton_app_cons in Ha as [He1' [Ht1 Ht2]].
+    rewrite Ht1 Ht2 in Hb. simpl in Hb.
+
+    inversion Hstep'''.
+    - inversion H.
+      all: rewrite -H7 in H3;
+             rewrite -He1' -H0 in He1;
+             apply fill_seq_instr in He1 as [Hk He1];
+             rewrite Hk -H3 in He2; simpl in He2;
+             rewrite He2 -H5 in Hb. 1,2,3: simplify_eq.
+      1,2,3: assert (IH: ∃ fuel : nat, machine_run fuel (Failed, σ2) = Some cf').
+      1,3,5: apply (IHl σ2 φ' Failed cf'); try auto;
+             intros i a' b' Hi Hsi; apply (Hstep (S i) a' b');
+             simpl; assumption.
+      1,2,3: destruct IH as [fuel Hmr]; exists (S fuel); simpl;
+             destruct σ2 as [r m].
+      + simpl in H8. rewrite H8.
+        destruct fuel; simpl in Hmr. discriminate.
+        apply Hmr.
+      + simpl in H9. rewrite H9.
+        rewrite -isCorrectPCb_nisCorrectPC in H10.
+        rewrite H10.
+        destruct fuel; simpl in Hmr. discriminate. apply Hmr.
+      + simpl in H9. rewrite H9. simpl in H10.
+        destruct (isCorrectPCb (WCap p b0 e a0)).
+        rewrite H10.
+        all: destruct fuel; simpl in Hmr; discriminate || apply Hmr.
+      + rewrite He1. rewrite He1 in He1' Hhd.
+        assert (IH: ∃ fuel : nat, machine_run fuel (c.1, σ2) = Some cf').
+        apply (IHl σ2 φ'). rewrite Hb. reflexivity.
+        auto. intros j a' b' Hi Hsi; apply (Hstep (S j) a' b');
+        simpl; assumption.
+        destruct IH as [fuel Hmr]; exists (S fuel); simpl.
+        rewrite Hφ. destruct σ1 as [r m].
+        rewrite -isCorrectPCb_isCorrectPC in H11.
+        rewrite -H12 in H13.
+        rewrite H9 H11 H10 H13 H8. apply Hmr.
+    - rewrite -He1' -H in He1. apply fill_seq_seq in He1.
+      destruct He1 as [HK Hcf].
+      rewrite HK in He2. simpl in He2.
+      rewrite Hcf.
+      rewrite He2 -H2 -H3 -H4 -Hφ in Hb.
+      specialize (IHl φ φ' Executable cf').
+      assert (IH: ∃ fuel : nat, machine_run fuel (Executable, φ) = Some cf').
+      { apply IHl. simpl. rewrite Hb. reflexivity.
+        apply Htl.
+        intros i a' b' Hi Hsi.
+        apply (Hstep (S i) a' b'); simpl; assumption. }
+      destruct IH as [fuel Hmr]. exists (S fuel). simpl. apply Hmr.
+    - rewrite -He1' -H in He1. apply fill_seq_seq in He1.
+      destruct He1 as [HK Hcf].
+      rewrite HK in He2. simpl in He2.
+      rewrite Hcf.
+      rewrite He2 -H2 -H3 -H4 -Hφ in Hb.
+      rewrite Hcf in He1', Hhd. rewrite Hhd in Hstep.
+      assert (cf' = Halted).
+      eapply erased_step_seq_halted.
+      apply rtc_list.
+      exists (([Seq (Instr Halted)], φ) :: b :: l).
+      split. reflexivity.
+      split. apply Htl. apply Hstep.
+      rewrite H5. exists 1. simpl. reflexivity.
+    - rewrite -He1' -H in He1. apply fill_seq_seq in He1.
+      destruct He1 as [HK Hcf].
+      rewrite HK in He2. simpl in He2.
+      rewrite Hcf.
+      rewrite He2 -H2 -H3 -H4 -Hφ in Hb.
+      rewrite Hcf in He1', Hhd. rewrite Hhd in Hstep.
+      assert (cf' = Failed).
+      eapply erased_step_seq_failed.
+      apply rtc_list.
+      exists (([Seq (Instr Failed)], φ) :: b :: l).
+      split. reflexivity.
+      split. apply Htl. apply Hstep.
+      rewrite H5. exists 1. simpl. reflexivity.
   Qed.
 
   Lemma machine_run_ends_in_halted_or_error:
